.

cfrontend/BeePL.v
@@ -1,7 +1,7 @@
 Require Import String ZArith Coq.FSets.FMapAVL Coq.Structures.OrderedTypeEx.
 Require Import Coq.FSets.FSetProperties Coq.FSets.FMapFacts FMaps FSetAVL Nat PeanoNat.
 Require Import Coq.Arith.EqNat Coq.ZArith.Int Integers AST Maps Globalenvs compcert.lib.Coqlib Ctypes.
-Require Import BeePL_aux BeeTypes Axioms Memory Int Cop Memtype Errors.
+Require Import BeePL_aux BeeTypes Axioms Memory Int Cop Memtype Errors Csem.
 From mathcomp Require Import all_ssreflect. 
 
 Set Implicit Arguments.
@@ -547,58 +547,6 @@ Section Small_step_semantics.
 Variable (ge: genv).
 Variable (vm : vmap). 
 
-Inductive lreduction : expr -> Memory.mem -> expr -> Memory.mem -> Prop :=
-| lred_var_local : forall hm x t l,
-                   vm!(x.(vname)) = Some (l, t) ->
-                   t = x.(vtype) ->
-                   lreduction (Var x) hm (Addr {| lname := l; ltype := t; lbitfield := Full |} Ptrofs.zero) hm
-| lred_var_global : forall hm x t l,
-                    vm!(x.(vname)) = None ->
-                    t = x.(vtype) ->
-                    Genv.find_symbol ge x.(vname) = Some l ->
-                    lreduction (Var x) hm (Addr {| lname := l; ltype := t; lbitfield := Full |} Ptrofs.zero) hm
-| lred_deref : forall hm l ofs tv t,
-               lreduction (Prim Deref (Val (Vloc l ofs) tv:: nil) t) hm 
-               (Addr {| lname := l; ltype := t; lbitfield := Full |} ofs) hm.
-
-Inductive rreduction : expr -> Memory.mem -> expr -> Memory.mem -> Prop :=
-| rred_valof : forall hm e t l ofs bf v,
-               deref_addr (typeof_expr e) hm l ofs bf v ->
-               typeof_expr e = t ->
-               BeeTypes.type_is_volatile t = false ->
-               rreduction (Valof (Addr {| lname := l; ltype := t; lbitfield := bf |} ofs) t) hm (Val v t) hm
-| rred_ref : forall hm v tv t hm' l, 
-             Mem.alloc hm 0 (sizeof_type tv) = (hm', l) ->
-             assign_addr tv hm' l Ptrofs.zero Full v hm' v ->
-             rreduction (Prim Ref [:: (Val v tv)] t) hm (Val (Vloc l Ptrofs.zero) tv) hm'
-| rred_uop : forall hm v t ct uop v' v'',
-             transBeePL_type t = OK ct ->
-             sem_unary_operation uop (transBeePL_value_cvalue v) ct hm = Some v' -> 
-             transC_val_bplvalue v' = OK v'' ->
-             rreduction (Prim (Uop uop) ((Val v t) :: nil) t) hm (Val v'' t) hm
-| rred_bop : forall hm bop v1 t1 v2 t2 ct1 ct2 t v v',
-             transBeePL_type t1 = OK ct1 ->
-             transBeePL_type t2 = OK ct2 ->
-             sem_binary_operation ge bop (transBeePL_value_cvalue v1) ct1 (transBeePL_value_cvalue v2) ct2 hm = Some v ->
-             transC_val_bplvalue v = OK v' ->
-             rreduction (Prim (Bop bop) ((Val v1 t1) :: (Val v2 t2) :: nil) t) hm (Val v' t) hm
-| rred_cond : forall hm v e1 e2 tv t ctv b, 
-              transBeePL_type tv = OK ctv ->
-              bool_val (transBeePL_value_cvalue v) ctv hm = Some b ->
-              rreduction (Cond (Val v tv) e1 e2 t) hm (if b then e1 else e2) hm
-| rred_massgn : forall hm l ofs v tv2 ct1 ct2 t hm' v' bf,
-                transBeePL_type t = OK ct1 ->
-                transBeePL_type tv2 = OK ct2 ->
-                sem_cast (transBeePL_value_cvalue v) ct2 ct1 hm = Some (transBeePL_value_cvalue v') ->
-                assign_addr t hm l ofs bf v' hm' v' ->
-                rreduction (Prim Massgn ((Addr {| lname := l; ltype := t; lbitfield := bf |} ofs) :: Val v tv2 :: nil) t) hm (Val v' t) hm'
-| rred_bind : forall vm hm x v e2 e2' t t' hm',
-              subst vm hm x v e2 hm' e2' ->
-              rreduction (Bind x t (Val v t) e2 t') hm e2' hm'
-| rred_unit : forall hm,
-              rreduction (Unit (Ptype Tunit)) hm (Val Vunit (Ptype Tunit)) hm.
-
- 
 Inductive is_list_val : list expr -> list value -> Prop :=
   | is_args_nil:
       is_list_val nil nil
@@ -612,17 +560,114 @@ Inductive callreduction : expr -> Memory.mem -> fundef -> list value -> type -> 
              type_of_fundef (Internal fd) ef = (Ftype ts ef rt) ->
              is_list_val vargs vargs' ->
              callreduction (App (Val v (Ftype ts ef rt)) vargs t) hm (Internal fd) vargs' t.
-  
+
+Inductive lreduction : expr -> Memory.mem -> expr -> Memory.mem -> Prop :=
+| lred_var_local : forall hm x t l,
+                   vm!(x.(vname)) = Some (l, t) ->
+                   t = x.(vtype) ->
+                   lreduction (Var x) hm (Addr {| lname := l; ltype := t; lbitfield := Full |} Ptrofs.zero) hm
+| lred_var_global : forall hm x t l,
+                    vm!(x.(vname)) = None ->
+                    t = x.(vtype) ->
+                    Genv.find_symbol ge x.(vname) = Some l ->
+                    lreduction (Var x) hm (Addr {| lname := l; ltype := t; lbitfield := Full |} Ptrofs.zero) hm
+| lred_deref : forall hm l ofs tv t,
+               lreduction (Prim Deref (Val (Vloc l ofs) tv:: nil) t) hm 
+               (Addr {| lname := l; ltype := t; lbitfield := Full |} ofs) hm
+| lred_deref1 : forall hm e e' t hm',
+                rreduction e hm e' hm' ->
+                lreduction (Prim Deref [:: e] t) hm  (Prim Deref [:: e'] t) hm'
+
+with rreduction : expr -> Memory.mem -> expr -> Memory.mem -> Prop :=
+| rred_valof : forall hm e t l ofs bf v,
+               deref_addr (typeof_expr e) hm l ofs bf v ->
+               typeof_expr e = t ->
+               BeeTypes.type_is_volatile t = false ->
+               rreduction (Valof (Addr {| lname := l; ltype := t; lbitfield := bf |} ofs) t) hm (Val v t) hm
+| rred_valof1 : forall hm e t e' hm',
+                lreduction e hm e' hm' ->
+                rreduction (Valof e t) hm (Valof e' t) hm'
+| rred_ref : forall hm v tv t hm' l, 
+             Mem.alloc hm 0 (sizeof_type tv) = (hm', l) ->
+             assign_addr tv hm' l Ptrofs.zero Full v hm' v ->
+             rreduction (Prim Ref [:: (Val v tv)] t) hm (Val (Vloc l Ptrofs.zero) tv) hm'
+| rred_ref1 : forall hm e t e' hm', 
+              rreduction e hm e' hm' ->
+              rreduction (Prim Ref [:: e] t) hm (Prim Ref [:: e] t) hm'
+| rred_uop : forall hm v t ct uop v' v'',
+             transBeePL_type t = OK ct ->
+             sem_unary_operation uop (transBeePL_value_cvalue v) ct hm = Some v' -> 
+             transC_val_bplvalue v' = OK v'' ->
+             rreduction (Prim (Uop uop) ((Val v t) :: nil) t) hm (Val v'' t) hm
+| rred_uop1 : forall hm t uop e e' hm',
+              rreduction e hm e' hm' ->
+              rreduction (Prim (Uop uop) (e :: nil) t) hm (Prim (Uop uop) (e' :: nil) t) hm'
+| rred_bop : forall hm bop v1 t1 v2 t2 ct1 ct2 t v v',
+             transBeePL_type t1 = OK ct1 ->
+             transBeePL_type t2 = OK ct2 ->
+             sem_binary_operation ge bop (transBeePL_value_cvalue v1) ct1 (transBeePL_value_cvalue v2) ct2 hm = Some v ->
+             transC_val_bplvalue v = OK v' ->
+             rreduction (Prim (Bop bop) ((Val v1 t1) :: (Val v2 t2) :: nil) t) hm (Val v' t) hm
+| rred_bop1 : forall hm t bop e1 e1' e2 hm',
+              rreduction e1 hm e1' hm' ->
+              rreduction (Prim (Bop bop) (e1 :: e2 :: nil) t) hm (Prim (Bop bop) (e1' :: e2 :: nil) t) hm'
+| rred_bop2 : forall hm bop v1 t1 t e2 e2' hm',
+              rreduction e2 hm e2' hm' ->
+              rreduction (Prim (Bop bop) ((Val v1 t1) :: e2 :: nil) t) hm (Prim (Bop bop) ((Val v1 t1) :: e2' :: nil) t) hm'
+| rred_cond : forall hm v e1 e2 tv t ctv b, 
+              transBeePL_type tv = OK ctv ->
+              bool_val (transBeePL_value_cvalue v) ctv hm = Some b ->
+              rreduction (Cond (Val v tv) e1 e2 t) hm (if b then e1 else e2) hm
+| rred_cond1 : forall hm e1 e2 e3 t e1' hm', 
+               rreduction e1 hm e1' hm' ->
+               rreduction (Cond e1 e2 e3 t) hm (Cond e1' e2 e3 t) hm
+| rred_massgn : forall hm l ofs v tv2 ct1 ct2 t hm' v' bf,
+                transBeePL_type t = OK ct1 ->
+                transBeePL_type tv2 = OK ct2 ->
+                sem_cast (transBeePL_value_cvalue v) ct2 ct1 hm = Some (transBeePL_value_cvalue v') ->
+                assign_addr t hm l ofs bf v' hm' v' ->
+                rreduction (Prim Massgn ((Addr {| lname := l; ltype := t; lbitfield := bf |} ofs) :: Val v tv2 :: nil) t) hm (Val v' t) hm'
+| rred_massgn1 : forall hm e1 e2 t e1' hm',
+                 rreduction e1 hm e1' hm' ->
+                 rreduction (Prim Massgn (e1 :: e2 :: nil) t) hm (Prim Massgn (e1' :: e2 :: nil) t) hm'
+| rred_massgn2 : forall hm l bf ofs e2 t e2' hm',
+                 rreduction e2 hm e2' hm' ->
+                 rreduction (Prim Massgn ((Addr {| lname := l; ltype := t; lbitfield := bf |} ofs) :: e2 :: nil) t) hm 
+                            (Prim Massgn ((Addr {| lname := l; ltype := t; lbitfield := bf |} ofs) :: e2' :: nil) t)  hm'
+| rred_bind : forall vm hm x v e2 e2' t t' hm',
+              subst vm hm x v e2 hm' e2' ->
+              rreduction (Bind x t (Val v t) e2 t') hm e2' hm'
+| rred_bind1 : forall hm x e1 e2 e1' t t' hm',
+               rreduction e1 hm e1' hm' ->
+               rreduction (Bind x t e1 e2 t') hm (Bind x t e1' e2 t') hm'
+| rred_app1 : forall hm e e' hm' es t,
+              rreduction e hm e' hm' ->
+              rreduction (App e es t) hm (App e' es t) hm'
+| rred_app2 : forall hm v ts ef rt es hm' es' t,
+              rreductions es hm es' hm' ->
+              rreduction (App (Val v (Ftype ts ef rt)) es t) hm (App (Val v (Ftype ts ef rt)) es t) hm'
+| rred_unit : forall hm,
+              rreduction (Unit (Ptype Tunit)) hm (Val Vunit (Ptype Tunit)) hm
+
+with rreductions : list expr -> Memory.mem -> list expr -> Memory.mem -> Prop :=
+| nil_rs : forall hm, rreductions nil hm nil hm
+| cons_rs : forall e es hm hm' hm'' e' es', 
+            rreduction e hm e' hm' ->
+            rreductions es hm' es' hm'' ->
+            rreductions (e :: es) hm (e' :: es') hm''.
+
+Scheme lreduction_mut := Minimality for lreduction Sort Prop
+  with rreduction_mut := Minimality for rreduction Sort Prop
+  with rreductions_mut := Minimality for rreductions Sort Prop.
+Combined Scheme lreduction_rreduction_rreductions_mut from lreduction_mut, rreduction_mut, rreductions_mut.
+
 (* Continuation describe the computations that remain to be performed 
    after the expression under consideration has evaluated completely *)
 Inductive cont: Type :=
 | Kstop : cont 
-| Kdo : cont -> cont          (* after [x] in [x;] *)
-| Klet : expr -> cont -> cont (* after x=e1 in bind x = e1 in e2) *)
-| Kcond : expr -> expr -> cont -> cont (* after [x] in if {x} {e1} {e2} *)
+| Kdo : cont -> cont  (* after [x] in [x;] *)
 | Kcall : function -> (* calling function *)
           vmap ->     (* local env of calling function *)
-          (expr -> expr) ->   (* context of the call *)
           type ->     (* type of call expression *)
           cont -> cont.          
 
@@ -642,127 +687,269 @@ Inductive state : Type :=
             (m : Memory.mem) : state
 | StuckState                          (* undefined behvaior occured *).
 
-(* Reduction contexts *)
-(* Kind can be a left value or a right value position representing the position of reduction *)
-Inductive kind : Type := LV | RV.
+(* Reduction contexts *) 
+Definition expr_kind (e: expr) : Csem.kind :=
+match e with
+| Val v t => RV 
+| Valof e t => RV 
+| Var v => LV
+| Const c t => RV
+| App e es t => RV
+| Prim b es t => match b with 
+                 | Ref => RV
+                 | Deref => LV
+                 | Massgn => RV 
+                 | Uop o => RV
+                 | Bop o => RV
+                 | Run h => RV (* Fix me *)
+                 end
+| Bind x t e e' t' => RV
+| Cond e1 e2 e3 t => RV
+| Unit t => RV
+| Addr l ofs => LV
+| Hexpr _ _ _ => RV (* Fix me *)
+end. 
 
-Inductive context : kind -> kind -> (expr -> expr) -> Prop :=
-| ctx_top : forall k,
-            context k k (fun x => x)
-(* Valof e t, where e is evaluated at LV position *)
-| ctx_valof : forall k C t,
-              context k LV C ->
-              context k RV (fun x => Valof (C x) t)
-(* Ref e t, where e is evaluated at RV position *)
-| ctx_ref : forall k C t,
-            context k RV C ->
-            context k RV (fun x => Prim Ref [:: C x] t)
-(* Deref e t, where e is evaluated at RV position, but deref is evaluated in LV *)
-| ctx_deref : forall k C t,
-              context k RV C ->
-              context k LV (fun x => Prim Deref [:: C x] t)
-(* e1 := e2, evaluates in two rules *)
-| ctx_massgn1 : forall k C t e2, 
-                context k LV C ->
-                context k RV (fun x => Prim Massgn (C x :: e2 :: nil) t)
-| ctx_massgn2 : forall k C t e1,
-                context k RV C ->
-                context k RV (fun x => Prim Massgn (e1 :: C x :: nil) t)
-(* uop(e), where e is evaluated at RV position *)
-| ctx_uop : forall k C t o,
-            context k RV C ->
-            context k RV (fun x => Prim (Uop o) [:: (C x)] t)
-(* bop(e1,e2), where e1 is evaluated at RV in first rule and e2 is evaluated at RV in second rule *)
-| ctx_bop1 : forall k C t o e2,
-             context k RV C ->
-             context k RV (fun x => Prim (Bop o) ((C x) :: e2 :: nil) t)
-| ctx_bop2 : forall k C t o e1,
-             context k RV C ->
-             context k RV (fun x => Prim (Bop o) (e1 :: (C x) :: nil) t)
-| ctx_cond : forall k C t e2 e3,
-             context k RV C ->
-             context k RV (fun x => Cond (C x) e2 e3 t)
-| ctx_bind : forall k C t r t' e,
-             context k RV C ->
-             context k RV (fun x => Bind r t' (C x) e t)
-| ctx_app1 : forall k C t es,
-             context k RV C ->
-             context k RV (fun x => App (C x) es t)
-| ctx_app2 : forall k C t e,
-             contexts k C ->
-             context k RV (fun x => App e (C x) t) 
-(* fix me : add the case for hexpr *)
-with contexts : kind -> (expr -> list expr) -> Prop :=
-| ctx_hd : forall k C el,
-           context k RV C ->
-           contexts k (fun x => (C x) :: el)
-| ctx_tl : forall k C e1,
-           contexts k C ->
-           contexts k (fun x => e1 :: (C x)).
+Definition is_lv (e : expr) : bool :=
+match e with 
+| Val v t => false 
+| Valof e t => false
+| Var v => true 
+| Const c t => false
+| App e es t => false 
+| Prim b es t => match b with 
+                 | Ref => false 
+                 | Deref => true 
+                 | Massgn => false
+                 | Uop o => false
+                 | Bop o => false
+                 | Run h => false (* fix me *)
+                 end
+| Bind x t e1 e2 t' => false
+| Cond e1 e2 e3 t => false
+| Unit t => false 
+| Addr l ofs => false
+| Hexpr m e t => false (* fix me *)
+end.
+
+Definition is_rv (e : expr) : bool :=
+match e with 
+| Val v t => true
+| Valof e t => true
+| Var v => false 
+| Const c t => true
+| App e es t => true 
+| Prim b es t => match b with 
+                 | Ref => true 
+                 | Deref => false 
+                 | Massgn => true
+                 | Uop o => true
+                 | Bop o => true
+                 | Run h => false (* fix me *)
+                 end
+| Bind x t e1 e2 t' => true
+| Cond e1 e2 e3 t => true
+| Unit t => true
+| Addr l ofs => false
+| Hexpr m e t => false (* fix me *)
+end.
+
+Section Is_reduced_forms.
+
+Variable is_reduced_form : expr -> bool.
+
+Fixpoint is_reduced_forms (es : list expr) : bool :=
+match es with 
+| nil => true 
+| e :: es => is_reduced_form e && is_reduced_forms es
+end.
+
+End Is_reduced_forms.
+
+Definition is_val (e : expr) : bool :=
+match e with 
+| Val v t => true 
+| _ => false
+end.
+
+Fixpoint is_vals (es : list expr) : bool :=
+match es with 
+| nil => true
+| e :: es => is_val e && is_vals es
+end.
+
+Fixpoint is_reduced_form (e : expr) : bool :=
+match e with 
+| Val v t => true 
+| Valof e t => is_reduced_form e
+| Var v => true 
+| Const c t => true 
+| App e es t => false 
+| Prim b es t => match b with 
+                 | Ref => is_reduced_forms is_reduced_form es 
+                 | Deref => is_vals es
+                 | Massgn => is_reduced_forms is_reduced_form es
+                 | Uop o => is_reduced_forms is_reduced_form es 
+                 | Bop o => is_reduced_forms is_reduced_form es 
+                 | Run h => false (* fix me *)
+                 end
+| Bind x t e1 e2 t' => is_reduced_form e1
+| Cond e1 e2 e3 t => is_reduced_form e1
+| Unit t => true 
+| Addr l ofs => true
+| Hexpr m e t => false (* fix me *)
+end.
+
               
 (* Relation representing safe execution of expressions *)
-Inductive expr_safe : kind -> expr -> Memory.mem -> Prop :=
-| expr_safe_val : forall v t m,
-                  expr_safe RV (Val v t) m
-| expr_safe_loc : forall l t m,
-                  expr_safe LV (Addr l t) m
-| expr_safe_lred : forall e m e' m' to C,
+Inductive expr_safe : expr -> Memory.mem -> Prop :=
+| expr_safe_lred : forall e m e' m',
                    lreduction e m e' m' ->
-                   context LV to C ->
-                   expr_safe to (C e) m
-| expr_safe_rred : forall e m e' m' to C,
+                   expr_safe e m
+| expr_safe_rred : forall e m e' m',
                    rreduction e m e' m' ->
-                   context RV to C -> 
-                   expr_safe to (C e) m
-| expr_safe_call : forall e m fd args t to C,
+                   expr_safe e m
+| expr_safe_call : forall e m fd args t,
                    callreduction e m fd args t ->
-                   context RV to C ->
-                   expr_safe to (C e) m.
+                   expr_safe e m.
 
 Definition not_stuck (e : expr) (m : Memory.mem) : Prop :=
-forall k C e',
-context k RV C -> e = C e' -> expr_safe k e' m.
+expr_safe e m.
 
 (* Reduction semantics *) 
 Inductive ssem : state -> state -> Prop :=
-| s_lreduction : forall C f e k e' m m',
+| s_lreduction : forall f e k e' m m',
                  lreduction e m e' m' ->
-                 context LV RV C ->
-                 ssem (ExprState f (C e) k vm m) (ExprState f (C e') k vm m')
-| s_rreduction : forall C f e k m e' m',
+                 ssem (ExprState f e k vm m) (ExprState f e' k vm m')
+| s_rreduction : forall f e k m e' m',
                  rreduction e m e' m' ->
-                 context RV RV C ->
-                 ssem (ExprState f (C e) k vm m) (ExprState f (C e') k vm m')
-| s_call : forall C f e k m fd args t,
+                 ssem (ExprState f e k vm m) (ExprState f e' k vm m')
+| s_call : forall f e k m fd args t,
            callreduction e m fd args t ->
-           context RV RV C ->
-           ssem (ExprState f (C e) k vm m) (CallState fd args (Kcall f vm C t k) m)
-| s_stuck : forall C f e k m K,
-            context K RV C ->
-            ~(expr_safe K e m) ->
-            ssem (ExprState f (C e) k vm m) StuckState
+           ssem (ExprState f e k vm m) (CallState fd args (Kcall f vm t k) m)
+| s_stuck : forall f e k m,
+            ~(expr_safe e m) ->
+            ssem (ExprState f e k vm m) StuckState
 | s_val : forall m k f v t,
           ssem (ExprState f (Val v t) (Kdo k) vm m) (ExprState f (Unit (Ptype Tunit)) k vm m)
 | s_internal_fun : forall f vargs k m m' m'',
                    list_norepet (f.(fn_args) ++ f.(fn_vars)) ->
                    alloc_variables empty_vmap m (f.(fn_args) ++ f.(fn_vars)) vm m' -> 
                    bind_variables vm m' f.(fn_args) vargs m'' ->
-                   ssem (CallState (Internal f) vargs k m) (ExprState f f.(fn_body) k vm m'')
-| s_cond1 : forall f e1 e2 e3 t k m,
-            ssem (ExprState f (Cond e1 e2 e3 t) k vm m) (ExprState f e1 (Kcond e2 e3 k) vm m)
-| s_cond2 : forall f v e2 e3 t k m ct b,
-            transBeePL_type t = OK ct ->
-            bool_val (transBeePL_value_cvalue v) ct m = Some b -> 
-            ssem (ExprState f (Val v t) (Kcond e2 e3 k) vm m) (ExprState f (if b then e2 else e3) k vm m)
-(* add one more rule for bind to evaluate e1 *)
-| s_bind1 : forall f x t' v e2 t k m e2' m',
-            subst vm m x v e2 m' e2' ->
-            ssem (ExprState f (Bind x t' (Val v t') e2 t) k vm m) (ExprState f e2' k vm m').
+                   ssem (CallState (Internal f) vargs k m) (ExprState f f.(fn_body) k vm m'').
 
 Definition step (s : state) (s' : state) : Prop :=
 ssem s s'.
 
 End Small_step_semantics.
+
+
+Section Lreduction_Rreduction_Mult.
+
+Variable (ge : genv).
+Variable (vm : vmap).
+
+Context (Plred : expr -> Memory.mem -> expr -> Memory.mem -> Prop).
+Context (Prred : expr -> Memory.mem -> expr -> Memory.mem -> Prop).
+Context (Prreds : list expr -> Memory.mem -> list expr -> Memory.mem -> Prop).
+Context (Plrvarl : forall hm x t l, 
+                   vm!(x.(vname)) = Some (l, t) ->
+                   t = x.(vtype) ->
+                   Plred (Var x) hm (Addr {| lname := l; ltype := t; lbitfield := Full |} Ptrofs.zero) hm).
+Context (Plrvarg : forall hm x t l,
+                   vm!(x.(vname)) = None ->
+                   t = x.(vtype) ->
+                   Genv.find_symbol ge x.(vname) = Some l ->
+                   Plred (Var x) hm (Addr {| lname := l; ltype := t; lbitfield := Full |} Ptrofs.zero) hm).
+Context (Plderef : forall hm l ofs tv t,
+                   Plred (Prim Deref (Val (Vloc l ofs) tv:: nil) t) hm (Addr {| lname := l; ltype := t; lbitfield := Full |} ofs) hm).
+Context (Plderef1 : forall hm e e' t hm',
+                    Prred e hm e' hm' ->
+                    Plred (Prim Deref [:: e] t) hm  (Prim Deref [:: e'] t) hm').
+Context (Prvalof : forall hm e t l ofs bf v,
+                   deref_addr (typeof_expr e) hm l ofs bf v ->
+                   typeof_expr e = t ->
+                   BeeTypes.type_is_volatile t = false ->
+                   Prred (Valof (Addr {| lname := l; ltype := t; lbitfield := bf |} ofs) t) hm (Val v t) hm).
+Context (Prvalof1 : forall hm e t e' hm',
+                    Plred e hm e' hm' ->
+                    Prred (Valof e t) hm (Valof e' t) hm').
+Context (Prref : forall hm v tv t hm' l, 
+                 Mem.alloc hm 0 (sizeof_type tv) = (hm', l) ->
+                 assign_addr tv hm' l Ptrofs.zero Full v hm' v ->
+                 Prred (Prim Ref [:: (Val v tv)] t) hm (Val (Vloc l Ptrofs.zero) tv) hm').
+Context (Prref1 : forall hm e t e' hm', 
+                  Prred e hm e' hm' ->
+                  Prred (Prim Ref [:: e] t) hm (Prim Ref [:: e] t) hm').
+Context (Pruop : forall hm v t ct uop v' v'',
+                 transBeePL_type t = OK ct ->
+                 sem_unary_operation uop (transBeePL_value_cvalue v) ct hm = Some v' -> 
+                 transC_val_bplvalue v' = OK v'' ->
+                 Prred (Prim (Uop uop) ((Val v t) :: nil) t) hm (Val v'' t) hm).
+Context (Pruop1 : forall hm t uop e e' hm',
+                  Prred e hm e' hm' ->
+                  Prred (Prim (Uop uop) (e :: nil) t) hm (Prim (Uop uop) (e' :: nil) t) hm').
+Context (Prbop : forall hm bop v1 t1 v2 t2 ct1 ct2 t v v',
+                 transBeePL_type t1 = OK ct1 ->
+                 transBeePL_type t2 = OK ct2 ->
+                 sem_binary_operation ge bop (transBeePL_value_cvalue v1) ct1 (transBeePL_value_cvalue v2) ct2 hm = Some v ->
+                 transC_val_bplvalue v = OK v' ->
+                 Prred (Prim (Bop bop) ((Val v1 t1) :: (Val v2 t2) :: nil) t) hm (Val v' t) hm).
+Context (Prbop1 : forall hm t bop e1 e1' e2 hm',
+                  Prred e1 hm e1' hm' ->
+                  Prred (Prim (Bop bop) (e1 :: e2 :: nil) t) hm (Prim (Bop bop) (e1' :: e2 :: nil) t) hm').
+Context (Prbop2 : forall hm bop v1 t1 t e2 e2' hm',
+                  Prred e2 hm e2' hm' ->
+                  Prred (Prim (Bop bop) ((Val v1 t1) :: e2 :: nil) t) hm (Prim (Bop bop) ((Val v1 t1) :: e2' :: nil) t) hm').
+Context (Prcond : forall hm v e1 e2 tv t ctv b, 
+                  transBeePL_type tv = OK ctv ->
+                  bool_val (transBeePL_value_cvalue v) ctv hm = Some b ->
+                  Prred (Cond (Val v tv) e1 e2 t) hm (if b then e1 else e2) hm).
+Context (Prcond1 : forall hm e1 e2 e3 t e1' hm', 
+                   Prred e1 hm e1' hm' ->
+                   Prred (Cond e1 e2 e3 t) hm (Cond e1' e2 e3 t) hm).
+Context (Prmassgn : forall hm l ofs v tv2 ct1 ct2 t hm' v' bf,
+                    transBeePL_type t = OK ct1 ->
+                    transBeePL_type tv2 = OK ct2 ->
+                    sem_cast (transBeePL_value_cvalue v) ct2 ct1 hm = Some (transBeePL_value_cvalue v') ->
+                    assign_addr t hm l ofs bf v' hm' v' ->
+                    Prred (Prim Massgn ((Addr {| lname := l; ltype := t; lbitfield := bf |} ofs) :: Val v tv2 :: nil) t) hm (Val v' t) hm').
+Context (Prmassgn1 : forall hm e1 e2 t e1' hm',
+                     Prred e1 hm e1' hm' ->
+                     Prred (Prim Massgn (e1 :: e2 :: nil) t) hm (Prim Massgn (e1' :: e2 :: nil) t) hm').
+Context (Prmassgn2 : forall hm l bf ofs e2 t e2' hm',
+                     Prred e2 hm e2' hm' ->
+                     Prred (Prim Massgn ((Addr {| lname := l; ltype := t; lbitfield := bf |} ofs) :: e2 :: nil) t) hm 
+                            (Prim Massgn ((Addr {| lname := l; ltype := t; lbitfield := bf |} ofs) :: e2' :: nil) t)  hm').
+Context (Prbind : forall vm hm x v e2 e2' t t' hm',
+                  subst vm hm x v e2 hm' e2' ->
+                  Prred (Bind x t (Val v t) e2 t') hm e2' hm').
+Context (Prbind1 : forall hm x e1 e2 e1' t t' hm',
+                   Prred e1 hm e1' hm' ->
+                   Prred (Bind x t e1 e2 t') hm (Bind x t e1' e2 t') hm').
+Context (Prapp1 : forall hm e e' hm' es t,
+                  Prred e hm e' hm' ->
+                  Prred (App e es t) hm (App e' es t) hm').
+Context (Prapp2 : forall hm v ts ef rt es hm' es' t,
+                  Prreds es hm es' hm' ->
+                  Prred (App (Val v (Ftype ts ef rt)) es t) hm (App (Val v (Ftype ts ef rt)) es t) hm').
+Context (Prunit : forall hm,
+                  Prred (Unit (Ptype Tunit)) hm (Val Vunit (Ptype Tunit)) hm).
+Context (Prnil : forall hm, Prreds nil hm nil hm).
+Context (Prcons : forall e es hm hm' hm'' e' es', 
+                  Prred e hm e' hm' ->
+                  Prreds es hm' es' hm'' ->
+                  Prreds (e :: es) hm (e' :: es') hm'').
+
+Lemma lreduction_rreduction_rreductions_ind : 
+(forall e hm e' hm', lreduction ge vm e hm e' hm' -> Plred e hm e' hm) /\
+(forall e hm e' hm', rreduction ge vm e hm e' hm' -> Prred e hm e' hm) /\
+(forall es hm es' hm', rreductions ge vm es hm es' hm' -> Prreds es hm es' hm).
+Proof.
+apply lreduction_rreduction_rreductions_mut=> //=.
+Admitted.
+
+End Lreduction_Rreduction_Mult.
 
 (* Whole program semantics *) (* Fix me *)
 (* Execution of whole program is defined as sequences of transition from initial state 
